# Basic Mathematics by Serge Lang

## Algebra

Numbers:
integers; used for counting
  positive, negative, and zero
positive integers
natural numbers; are positive integers and zero
0 is called the origin
negative integers; go below zero

0 + a = a + 0 = a
a + (-a) = 0 and -a + a = 0
  minus a (-a)
  -a is the additive inverse of a.

the sum and product of integers are also integers.

Rules for addition:
commutativity; 
  if a, b are integers, then;
    a + b = b + a 
  also holds with negative numbers
Associativity:
  if a, b, c are integers, then;
    (a + b) + c = a + (b + c)
      a + b + c
  also holds with negative numbers

if a + b = 0, then b = -a and a = -b
  a - b = a + (-b)
(a - b) + c = (a + (-b)) + c
  = a + (-b + c) by associativity
  = a + (c - b) by commutativity
  = (a + c) -b by associativity
  a - b + c = a + c - b by omitting the parentheses.

a = - (-a)
  if a is positive, the -a is negative
  if a is negative, the -a is positive

-( a + b) = -a + (-b)
-( a + b) = -a - b
  (a + b) + (-a -b) = 0
  (a + b) + (-a -b) = a + b -a -b by associativity
    = a - a + b - b by commutativity
    = 0 + 0
    = 0

-(-a) = a
if a, b are positive integers, then a + b is positive.
if a, b are negative integers, then a + b is negative.
a + b = c
  a = c - b
  b = c - a

Rules for Multiplication:
product of two integers is a integer
commutativity: ab = ba
associativity: (ab)c = a(bc)
1a = a
0a = 0
distributivity: a(b + c) = ab + ac and (b + c)a = ba + ca
  (b + c)a = a(b + c) = ab + ac = ba + bc
(-1)a = -a
-(ab) = (-a)b
-(ab) = a(-b)
(-a)(-b) = ab
$a^{m \times n}$

$aa = a^{2}$
$aaa = a^{3}$
$aaaa = a^{4}$
$a^{n} = aa...a \text{ (the product is taken n times).}$
$a^{n}$ is the n-the power of a
  $a^{2}$ is the second power of a
  $a^{5}$ is the fifth power of a
$a^{m+n} = a^{m}a^{n}$
  if m,n are positive integers
  $a^{2}a^{3} = (aa)(aaa) = a^{2+3} = aaaaa = a^{5}$
$(a^m)^n = a^{mn}$
$(ab)^n = a^nb^n$
  product of ab with itself n times
  $(2a^3)^5 = 2^5(a^3)^5 = 32a^{15}$

$(a + b)^2 = a^2 + 2ab + b^2$
$(a - b)^2 = a^2 - 2ab + b^2$
$(a + b)(a - b) = a^2 - b^2$
$(a + b)^2 = (a + b)(a + b) = a(a + b) + b(a + b) = a^2 + ab + ba + b^2
= a^2 + 2ab + b^2$
$(a - b)^2 = (a - b)(a - b)$
  $= a(a-b) - b(a-b)$
  $= aa-ab -ba+bb$
  $= a^2 -2ab + b^2$
$(a+b)(a-b)=a(a-b)+b(a-b)=aa-ab+ba-bb$
  $=a^2-b^2$
  $= aa-ab -ba-bb$
